%! TeX root = ../../main.tex

\chapter{Fourier transform}
\label{app:fourier-transform}

Fourier transform of the retarded correlator from time to frequency space.
\begin{align}
    C_z
     & =
    -\mi \Theta(t) \langle \{A(t), B\}\rangle                                 \\
     & =
    -\mi \Theta(t) \langle A(t) B\rangle -\mi \Theta(t) \langle B A(t)\rangle \\
     & =
    C^+_z + C^-_z
\end{align}
Transformation of the first component:
\begin{align}
    C^+_z
     & =
    \int_{-\infty}^\infty \md t \>
    \me^{\mi zt}(-\mi \Theta(t) \langle \me^{\mi Ht} A \me^{-\mi Ht} B\rangle)     \\
     & =
    -\mi \int_0^\infty \md t \>
    \me^{\mi zt} \langle \me^{\mi Ht} A \me^{-\mi Ht} B\rangle                     \\
     & =
    -\mi \int_0^\infty \md t \>
    \me^{\mi zt} \langle \me^{\mi E_0t} A \me^{-\mi Ht} B\rangle                   \\
     & =
    -\mi \int_0^\infty \md t \>
    \langle A \me^{\mi(z - H + E_0)t} B\rangle                                     \\
     & =
    -\mi \left.\left\langle A \frac{\me^{\mi(z - H + E_0)t}}{\mi(z - H + E_0)} B\right\rangle
    \right|_0^\infty                                                               \\
     & =
    -\mi \left(0 - \left\langle A \frac{1}{\mi(z - H + E_0)} B\right\rangle\right) \\
     & =
    \left\langle A \frac{1}{z - H + E_0} B\right\rangle
\end{align}
Transformation of the second component:
\begin{align}
    C^-_z
     & =
    \int_{-\infty}^\infty \md t \>
    \me^{\mi zt}(-\mi \Theta(t) \langle B \me^{\mi Ht} A \me^{-\mi Ht}\rangle) \\
     & =
    -\mi \int_0^\infty \md t \>
    \me^{\mi zt} \langle B \me^{\mi Ht} A \me^{-\mi Ht}\rangle                 \\
     & =
    -\mi \int_0^\infty \md t \>
    \me^{\mi zt} \langle B \me^{\mi Ht} A \me^{-\mi E_0t}\rangle               \\
     & =
    -\mi \int_0^\infty \md t \>
    \langle B \me^{\mi(z + H - E_0)t} A\rangle                                 \\
     & =
    \left\langle B \frac{1}{z + H - E_0} A\right\rangle
\end{align}
